Updates.

HandbookOfPracticalLogicLean/Chapter2.lean
@@ -1,5 +1,7 @@
 import MathlibExtraLean.FunctionUpdateITE
 
+import HandbookOfPracticalLogicLean.Chapter2.Formula
+
 import Lean
 import Batteries.Tactic.Lint.Frontend
 import Mathlib.Util.CompileInductive
@@ -9,173 +11,20 @@ import Mathlib.Tactic
 set_option autoImplicit false
 
 
-/--
-  The type of formulas.
--/
-inductive Formula_ : Type
-  | false_ : Formula_
-  | true_ : Formula_
-  | atom_ : String → Formula_
-  | not_ : Formula_ → Formula_
-  | and_ : Formula_ → Formula_ → Formula_
-  | or_ : Formula_ → Formula_ → Formula_
-  | imp_ : Formula_ → Formula_ → Formula_
-  | iff_ : Formula_ → Formula_ → Formula_
-  | forall_ : String → Formula_ → Formula_
-  | exists_ : String → Formula_ → Formula_
-  deriving Inhabited, DecidableEq, Repr
-
-compile_inductive% Formula_
-
-
-/--
-  The string representation of formulas.
--/
-def Formula_.toString :
-  Formula_ → String
-  | false_ => "F."
-  | true_ => "T."
-  | atom_ X => s! "{X}"
-  | not_ phi => s! "(¬ {phi.toString})"
-  | and_ phi psi => s! "({phi.toString} ∧ {psi.toString})"
-  | or_ phi psi => s! "({phi.toString} ∨ {psi.toString})"
-  | imp_ phi psi => s! "({phi.toString} → {psi.toString})"
-  | iff_ phi psi => s! "({phi.toString} ↔ {psi.toString})"
-  | forall_ x phi => s! "(∀. {x} {phi.toString})"
-  | exists_ x phi => s! "(∃. {x} {phi.toString})"
-
-instance : ToString Formula_ :=
-  { toString := Formula_.toString }
-
-#eval (Formula_.atom_ "P").toString
-
-
-open Lean Elab Meta
-
-declare_syntax_cat formula
-
-
-syntax "F." : formula
-syntax "T." : formula
-syntax ident : formula
-syntax "~" formula : formula
-syntax "(" formula "/\\" formula ")" : formula
-syntax "(" formula "\\/" formula ")" : formula
-syntax "(" formula "->" formula ")" : formula
-syntax "(" formula "<->" formula ")" : formula
-syntax "(" "A." ident formula ")" : formula
-syntax "(" "E." ident formula ")" : formula
-
-
-partial def elabFormula : Syntax → MetaM Expr
-  | `(formula| F.) => mkAppM ``Formula_.false_ #[]
-
-  | `(formula| T.) => mkAppM ``Formula_.true_ #[]
-
-  | `(formula| $X:ident) => do
-    let X' : Expr := Lean.mkStrLit X.getId.toString
-    mkAppM ``Formula_.atom_ #[X']
-
-  | `(formula| ~ $phi) => do
-    let phi' : Expr ← elabFormula phi
-    mkAppM ``Formula_.not_ #[phi']
-
-  | `(formula| ($phi:formula /\ $psi:formula)) => do
-    let phi' : Expr ← elabFormula phi
-    let psi' : Expr ← elabFormula psi
-    mkAppM ``Formula_.and_ #[phi', psi']
-
-  | `(formula| ($phi:formula \/ $psi:formula)) => do
-    let phi' : Expr ← elabFormula phi
-    let psi' : Expr ← elabFormula psi
-    mkAppM ``Formula_.or_ #[phi', psi']
-
-  | `(formula| ($phi:formula -> $psi:formula)) => do
-    let phi' : Expr ← elabFormula phi
-    let psi' : Expr ← elabFormula psi
-    mkAppM ``Formula_.imp_ #[phi', psi']
-
-  | `(formula| ($phi:formula <-> $psi:formula)) => do
-    let phi' : Expr ← elabFormula phi
-    let psi' : Expr ← elabFormula psi
-    mkAppM ``Formula_.iff_ #[phi', psi']
-
-  | `(formula| (A. $x:ident $phi)) => do
-    let x' : Expr := Lean.mkStrLit x.getId.toString
-    let phi' : Expr ← elabFormula phi
-    mkAppM ``Formula_.forall_ #[x', phi']
-
-  | `(formula| (E. $x:ident $phi)) => do
-    let x' : Expr := Lean.mkStrLit x.getId.toString
-    let phi' : Expr ← elabFormula phi
-    mkAppM ``Formula_.exists_ #[x', phi']
-
-  | _ => throwUnsupportedSyntax
-
-
-elab "(Formula_|" p:formula ")" : term => elabFormula p
-
-
-#check (Formula_| F. )
-#check (Formula_| T. )
-#check (Formula_| P )
-#check (Formula_| ~ P )
-#check (Formula_| (P /\ Q) )
-#check (Formula_| (P \/ Q) )
-#check (Formula_| (P -> Q) )
-#check (Formula_| (P <-> Q) )
-#check (Formula_| ( A. x P ) )
-#check (Formula_| ( E. x P ) )
-
-
 open Formula_
-
-def Formula_.map_atoms
-  (f : String → Formula_) :
-  Formula_ → Formula_
-  | false_ => false_
-  | true_ => true_
-  | atom_ X => f X
-  | not_ phi => not_ (phi.map_atoms f)
-  | and_ phi psi => and_ (phi.map_atoms f) (psi.map_atoms f)
-  | or_ phi psi => or_ (phi.map_atoms f) (psi.map_atoms f)
-  | imp_ phi psi => imp_ (phi.map_atoms f) (psi.map_atoms f)
-  | iff_ phi psi => iff_ (phi.map_atoms f) (psi.map_atoms f)
-  | forall_ x phi => forall_ x (phi.map_atoms f)
-  | exists_ x phi => forall_ x (phi.map_atoms f)
-
-
--- Applies function f to all of the atoms of the formula, from right to left.
-def Formula_.foldr_atoms
-  {α : Type}
-  (f : String → α → α)
-  (init : α) :
-  Formula_ → α
-  | false_
-  | true_ => init
-  | atom_ X => f X init
-  | not_ phi => phi.foldr_atoms f init
-  | and_ phi psi
-  | or_ phi psi
-  | imp_ phi psi
-  | iff_ phi psi => phi.foldr_atoms f (psi.foldr_atoms f init)
-  | forall_ _ phi
-  | exists_ _ phi => phi.foldr_atoms f init
 
 
 def atom_occurs_in
   (A : String) :
   Formula_ → Prop
-  | false_
+  | false_ => False
   | true_ => False
   | atom_ X => A = X
   | not_ phi => atom_occurs_in A phi
-  | and_ phi psi
-  | or_ phi psi
-  | imp_ phi psi
+  | and_ phi psi => atom_occurs_in A phi ∨ atom_occurs_in A psi
+  | or_ phi psi => atom_occurs_in A phi ∨ atom_occurs_in A psi
+  | imp_ phi psi => atom_occurs_in A phi ∨ atom_occurs_in A psi
   | iff_ phi psi => atom_occurs_in A phi ∨ atom_occurs_in A psi
-  | forall_ _ phi
-  | exists_ _ phi => atom_occurs_in A phi
 
 
 def PropValuation : Type := String → Prop
@@ -193,8 +42,6 @@ def eval
   | or_ phi psi => eval V phi ∨ eval V psi
   | imp_ phi psi => eval V phi → eval V psi
   | iff_ phi psi => eval V phi ↔ eval V psi
-  | forall_ _ phi
-  | exists_ _ phi => eval V phi
 
 instance
   (V : PropValuation)
@@ -206,87 +53,6 @@ instance
   all_goals
     simp only [eval]
     infer_instance
-
-
-def eval_opt
-  (V : PropValuation) :
-  Formula_ → Option Prop
-  | false_ => some False
-  | true_ => some True
-  | atom_ X => some (V X)
-  | not_ phi => do
-    let val_phi ← eval_opt V phi
-    ¬ val_phi
-  | and_ phi psi => do
-    let val_phi ← eval_opt V phi
-    let val_psi ← eval_opt V psi
-    val_phi ∧ val_psi
-  | or_ phi psi => do
-    let val_phi ← eval_opt V phi
-    let val_psi ← eval_opt V psi
-    val_phi ∨ val_psi
-  | imp_ phi psi => do
-    let val_phi ← eval_opt V phi
-    let val_psi ← eval_opt V psi
-    val_phi → val_psi
-  | iff_ phi psi => do
-    let val_phi ← eval_opt V phi
-    let val_psi ← eval_opt V psi
-    val_phi ↔ val_psi
-  | forall_ _ _
-  | exists_ _ _ => none
-
-
-def Formula_.is_prop :
-  Formula_ → Prop
-  | false_
-  | true_
-  | atom_ _ => True
-  | not_ phi => phi.is_prop
-  | and_ phi psi
-  | or_ phi psi
-  | imp_ phi psi
-  | iff_ phi psi => phi.is_prop ∧ psi.is_prop
-  | forall_ _ _
-  | exists_ _ _ => False
-
-
-lemma is_prop_imp_eval_opt_eq_some_eval
-  (F : Formula_)
-  (V : PropValuation)
-  (h1 : F.is_prop) :
-  eval_opt V F = some (eval V F) :=
-  by
-  induction F
-  case false_ | true_ | atom_ X =>
-    unfold eval_opt
-    unfold eval
-    rfl
-  case not_ phi ih =>
-    unfold is_prop at h1
-
-    simp only [eval_opt]
-    rewrite [ih h1]
-    simp only [eval]
-    simp
-  case
-      and_ phi psi phi_ih psi_ih
-    | or_ phi psi phi_ih psi_ih
-    | imp_ phi psi phi_ih psi_ih
-    | iff_ phi psi phi_ih psi_ih =>
-    unfold is_prop at h1
-    obtain ⟨h1_left, h1_right⟩ := h1
-
-    simp only [eval_opt]
-    rewrite [phi_ih h1_left]
-    rewrite [psi_ih h1_right]
-    simp only [eval]
-    simp
-  case
-      forall_ x phi ih
-    | exists_ x phi ih =>
-      unfold is_prop at h1
-      contradiction
 
 
 theorem theorem_2_2
@@ -329,13 +95,6 @@ theorem theorem_2_2
       unfold atom_occurs_in
       right
       exact a1
-  case
-      forall_ x phi phi_ih
-    | exists_ x phi phi_ih =>
-    unfold atom_occurs_in at h1
-
-    apply phi_ih
-    exact h1
 
 
 def satisfies
@@ -451,8 +210,6 @@ def replace_atom_one_rec
   | or_ phi psi => or_ (replace_atom_one_rec A F phi) (replace_atom_one_rec A F psi)
   | imp_ phi psi => imp_ (replace_atom_one_rec A F phi) (replace_atom_one_rec A F psi)
   | iff_ phi psi => iff_ (replace_atom_one_rec A F phi) (replace_atom_one_rec A F psi)
-  | forall_ x phi => forall_ x (replace_atom_one_rec A F phi)
-  | exists_ x phi => exists_ x (replace_atom_one_rec A F phi)
 
 
 theorem theorem_2_3_one
@@ -485,12 +242,6 @@ theorem theorem_2_3_one
     simp only [eval]
     rewrite [phi_ih]
     rewrite [psi_ih]
-    rfl
-  case
-      forall_ x phi phi_ih
-    | exists_ x phi phi_ih =>
-    simp only [eval]
-    rewrite [phi_ih]
     rfl
 
 
@@ -552,8 +303,6 @@ def replace_atom_all_rec
   | or_ phi psi => or_ (replace_atom_all_rec τ phi) (replace_atom_all_rec τ psi)
   | imp_ phi psi => imp_ (replace_atom_all_rec τ phi) (replace_atom_all_rec τ psi)
   | iff_ phi psi => iff_ (replace_atom_all_rec τ phi) (replace_atom_all_rec τ psi)
-  | forall_ x phi => forall_ x (replace_atom_all_rec τ phi)
-  | exists_ x phi => exists_ x (replace_atom_all_rec τ phi)
 
 
 theorem theorem_2_3_all
@@ -581,12 +330,6 @@ theorem theorem_2_3_all
     simp only [eval]
     rewrite [phi_ih]
     rewrite [psi_ih]
-    rfl
-  case
-      forall_ x phi phi_ih
-    | exists_ x phi phi_ih =>
-    simp only [eval]
-    rewrite [phi_ih]
     rfl
 
 
@@ -664,14 +407,6 @@ def is_repl_of_formula_in_formula_fun
     iff_ P_u Q_u = iff_ P_v Q_v ∨ (iff_ P_u Q_u = U ∧ iff_ P_v Q_v = V) ∨
     is_repl_of_formula_in_formula_fun U V P_u P_v ∧ is_repl_of_formula_in_formula_fun U V Q_u Q_v
 
-  | forall_ x_u P_u, forall_ x_v P_v =>
-    forall_ x_u P_u = forall_ x_v P_v ∨ (forall_ x_u P_u = U ∧ forall_ x_v P_v = V) ∨
-    (x_u = x_v ∧ is_repl_of_formula_in_formula_fun U V P_u P_v)
-
-  | exists_ x_u P_u, exists_ x_v P_v =>
-    exists_ x_u P_u = exists_ x_v P_v ∨ (exists_ x_u P_u = U ∧ exists_ x_v P_v = V) ∨
-    (x_u = x_v ∧ is_repl_of_formula_in_formula_fun U V P_u P_v)
-
   | P_u, P_v => P_u = P_v ∨ (P_u = U ∧ P_v = V)
 
 instance (U V F F' : Formula_) : Decidable (is_repl_of_formula_in_formula_fun U V F F') :=
@@ -682,9 +417,6 @@ instance (U V F F' : Formula_) : Decidable (is_repl_of_formula_in_formula_fun U 
     all_goals
       simp only [is_repl_of_formula_in_formula_fun]
       infer_instance
-
-
-#eval is_repl_of_formula_in_formula_fun (Formula_| (P /\ Q)) (Formula_| R) (Formula_| ((P /\ Q) /\ (P /\ Q))) (Formula_| (R /\ (P /\ Q)))
 
 
 /--
@@ -739,20 +471,6 @@ inductive is_repl_of_formula_in_formula
     is_repl_of_formula_in_formula U V P_u P_v →
     is_repl_of_formula_in_formula U V Q_u Q_v →
     is_repl_of_formula_in_formula U V (P_u.iff_ Q_u) (P_v.iff_ Q_v)
-
-  | forall_
-    (x_u x_v : String)
-    (P_u P_v : Formula_) :
-    x_u = x_v →
-    is_repl_of_formula_in_formula U V P_u P_v →
-    is_repl_of_formula_in_formula U V (forall_ x_u P_u) (forall_ x_v P_v)
-
-  | exists_
-    (x_u x_v : String)
-    (P_u P_v : Formula_) :
-    x_u = x_v →
-    is_repl_of_formula_in_formula U V P_u P_v →
-    is_repl_of_formula_in_formula U V (exists_ x_u P_u) (exists_ x_v P_v)
 
 
 lemma is_repl_of_formula_in_formula_fun_imp_is_repl_of_formula_in_formula
@@ -825,30 +543,6 @@ lemma is_repl_of_formula_in_formula_fun_imp_is_repl_of_formula_in_formula
         · apply phi_ih
           exact h1_left
         · apply psi_ih
-          exact h1_right
-  case
-      forall_.forall_ x phi ih x' phi'
-    | exists_.exists_ x phi ih x' phi' =>
-    unfold is_repl_of_formula_in_formula_fun at h1
-    cases h1
-    case inl h1 =>
-      apply is_repl_of_formula_in_formula.same_
-      exact h1
-    case inr h1 =>
-      cases h1
-      case inl h1 =>
-        obtain ⟨h1_left, h1_right⟩ := h1
-        apply is_repl_of_formula_in_formula.diff_
-        · exact h1_left
-        · exact h1_right
-      case inr h1 =>
-        obtain ⟨h1_left, h1_right⟩ := h1
-
-        first
-          | apply is_repl_of_formula_in_formula.forall_
-          | apply is_repl_of_formula_in_formula.exists_
-        · exact h1_left
-        · apply ih
           exact h1_right
 
   all_goals
@@ -928,12 +622,6 @@ example
     rewrite [ih_3]
     rewrite [ih_4]
     rfl
-  case
-      forall_ x_u x_v P_u P_v ih_1 ih_2 ih_3
-    | exists_ x_u x_v P_u P_v ih_1 ih_2 ih_3 =>
-    unfold eval
-    rewrite [ih_3]
-    rfl
 
 
 def Formula_.has_dual :
@@ -966,8 +654,6 @@ def Formula_.dual :
   | or_ phi psi => and_ phi.dual psi.dual
   | imp_ phi psi => imp_ phi.dual psi.dual
   | iff_ phi psi => iff_ phi.dual psi.dual
-  | forall_ x phi => forall_ x phi.dual
-  | exists_ x phi => exists_ x phi.dual
 
 
 example
@@ -987,11 +673,6 @@ example
     | iff_ phi psi phi_ih psi_ih =>
     rewrite [phi_ih]
     rewrite [psi_ih]
-    rfl
-  case
-      forall_ x phi ih
-    | exists_ x phi ih =>
-    rewrite [ih]
     rfl
 
 
@@ -1132,12 +813,6 @@ def is_subformula
     F = iff_ phi psi ∨
     is_subformula F phi ∨
     is_subformula F psi
-  | forall_ x phi =>
-    F = forall_ x phi ∨
-    is_subformula F phi
-  | exists_ x phi =>
-    F = exists_ x phi ∨
-    is_subformula F phi
 
 instance
   (F F' : Formula_) :
@@ -1302,7 +977,7 @@ lemma simplify_aux_is_logically_equivalent
   eval V F ↔ eval V (simplify_aux F) :=
   by
   cases F
-  case false_ | true_ | atom_ X | forall_ x phi | exists_ x phi =>
+  case false_ | true_ | atom_ X =>
     simp only [simplify_aux]
   case not_ phi =>
     cases phi
@@ -1343,7 +1018,7 @@ lemma simplify_is_logically_equivalent
   eval V F ↔ eval V (simplify F) :=
   by
   induction F
-  case false_ | true_ | atom_ X | forall_ x phi ih | exists_ x phi ih =>
+  case false_ | true_ | atom_ X =>
     rfl
   case not_ phi ih =>
     simp only [simplify]
@@ -1452,7 +1127,7 @@ theorem eval_to_nnf_neg_iff_not_eval_to_nnf_v1
     simp only [to_nnf_neg_v1]
     simp only [eval]
     tauto
-  case atom_ X | forall_ x phi ih | exists_ x phi ih =>
+  case atom_ X =>
     simp only [to_nnf_v1]
     simp only [to_nnf_neg_v1]
     simp only [eval]
@@ -1480,7 +1155,7 @@ example
   eval V F ↔ eval V (to_nnf_v1 F) :=
   by
   induction F
-  case false_ | true_ | atom_ X | forall_ x phi ih | exists_ x phi ih =>
+  case false_ | true_ | atom_ X =>
     unfold to_nnf_v1
     rfl
   case not_ phi ih =>
@@ -1523,7 +1198,7 @@ lemma to_nnf_neg_is_nnf_iff_to_nnf_is_nnf_v1
   (to_nnf_neg_v1 F).is_nnf ↔ (to_nnf_v1 F).is_nnf :=
   by
   induction F
-  case true_ | false_ | atom_ X | forall_ x phi ih | exists_ x phi ih =>
+  case true_ | false_ | atom_ X =>
     simp only [to_nnf_v1]
     simp only [to_nnf_neg_v1]
     simp only [is_nnf]
@@ -1544,8 +1219,7 @@ lemma to_nnf_neg_is_nnf_iff_to_nnf_is_nnf_v1
 
 
 example
-  (F : Formula_)
-  (h1 : F.is_prop) :
+  (F : Formula_) :
   (to_nnf_v1 F).is_nnf :=
   by
   induction F
@@ -1554,38 +1228,25 @@ example
     unfold is_nnf
     exact trivial
   case not_ phi ih =>
-    simp only [is_prop] at h1
-
     simp only [to_nnf_v1]
     rewrite [to_nnf_neg_is_nnf_iff_to_nnf_is_nnf_v1]
     apply ih
-    exact h1
   case
       and_ phi psi phi_ih psi_ih
     | or_ phi psi phi_ih psi_ih =>
-    simp only [is_prop] at h1
-
     simp only [to_nnf_v1]
     simp only [is_nnf]
     tauto
   case imp_ phi psi phi_ih psi_ih =>
-    simp only [is_prop] at h1
-
     simp only [to_nnf_v1]
     simp only [is_nnf]
     rewrite [to_nnf_neg_is_nnf_iff_to_nnf_is_nnf_v1]
     tauto
   case iff_ phi psi phi_ih psi_ih =>
-    simp only [is_prop] at h1
-
     simp only [to_nnf_v1]
     simp only [is_nnf]
     simp only [to_nnf_neg_is_nnf_iff_to_nnf_is_nnf_v1]
     tauto
-  case
-      forall_ x phi ih
-    | exists_ x phi ih =>
-    simp only [is_prop] at h1
 
 
 -------------------------------------------------------------------------------
@@ -1628,7 +1289,7 @@ theorem eval_to_nnf_neg_iff_not_eval_to_nnf_v2
     simp only [to_nnf_v2]
     simp only [to_nnf_neg_v2]
     simp only [eval]
-  case atom_ X | forall_ x phi ih | exists_ x phi ih =>
+  case atom_ X =>
     simp only [to_nnf_v2]
     simp only [to_nnf_neg_v2]
     simp only [eval]
@@ -1656,7 +1317,7 @@ example
   eval V F ↔ eval V (to_nnf_v2 F) :=
   by
   induction F
-  case false_ | true_ | atom_ X | forall_ x phi ih | exists_ x phi ih =>
+  case false_ | true_ | atom_ X =>
     unfold to_nnf_v2
     rfl
   case not_ phi ih =>
@@ -1707,7 +1368,7 @@ lemma to_nnf_neg_is_nnf_iff_to_nnf_is_nnf_v2
   case true_ =>
     simp only [is_subformula] at h2
     contradiction
-  case atom_ X | forall_ x phi ih | exists_ x phi ih =>
+  case atom_ X =>
     simp only [to_nnf_v2]
     simp only [to_nnf_neg_v2]
     simp only [is_nnf]
@@ -1732,7 +1393,6 @@ lemma to_nnf_neg_is_nnf_iff_to_nnf_is_nnf_v2
 
 example
   (F : Formula_)
-  (h1 : F.is_prop)
   (h2 : ¬ is_proper_subformula false_ F)
   (h3 : ¬ is_proper_subformula true_ F) :
   (to_nnf_v2 F).is_nnf :=
@@ -1743,8 +1403,6 @@ example
     unfold is_nnf
     exact trivial
   case not_ phi ih =>
-    simp only [is_prop] at h1
-
     simp only [is_proper_subformula] at h2
     simp only [is_subformula] at h2
 
@@ -1753,7 +1411,7 @@ example
 
     simp only [to_nnf_v2]
     rewrite [to_nnf_neg_is_nnf_iff_to_nnf_is_nnf_v2]
-    apply ih h1
+    apply ih
     · simp only [is_proper_subformula]
       tauto
     · simp only [is_proper_subformula]
@@ -1763,8 +1421,6 @@ example
   case
       and_ phi psi phi_ih psi_ih
     | or_ phi psi phi_ih psi_ih =>
-    simp only [is_prop] at h1
-
     simp only [is_proper_subformula] at h2
     simp only [is_subformula] at h2
 
@@ -1778,8 +1434,6 @@ example
     simp only [is_nnf]
     tauto
   case imp_ phi psi phi_ih psi_ih =>
-    simp only [is_prop] at h1
-
     simp only [is_proper_subformula] at h2
     simp only [is_subformula] at h2
 
@@ -1795,8 +1449,6 @@ example
     all_goals
       tauto
   case iff_ phi psi phi_ih psi_ih =>
-    simp only [is_prop] at h1
-
     simp only [is_proper_subformula] at h2
     simp only [is_subformula] at h2
 
@@ -1812,30 +1464,19 @@ example
     rewrite [to_nnf_neg_is_nnf_iff_to_nnf_is_nnf_v2]
     all_goals
       tauto
-  case
-      forall_ x phi ih
-    | exists_ x phi ih =>
-    simp only [is_prop] at h1
 
 
 -------------------------------------------------------------------------------
 
-/-
+
 example
-  (F : Formula_)
-  (h1 : F.is_prop) :
+  (F : Formula_) :
   ¬ is_proper_subformula false_ (simplify F) ∧
   ¬ is_proper_subformula true_ (simplify F) :=
   by
   induction F
   case and_ phi psi phi_ih psi_ih =>
-    simp only [is_prop] at h1
-    obtain ⟨h1_left, h1_right⟩ := h1
-
     simp only [simplify]
-    specialize phi_ih h1_left
-    specialize psi_ih h1_right
-
     simp only [is_proper_subformula] at phi_ih
 
     have s1 : simplify phi = true_ ∨ ¬ is_subformula true_ (simplify phi) :=
@@ -1996,4 +1637,5 @@ example
               simp only [is_subformula]
               tauto
     · sorry
--/
+  all_goals
+    sorry
