HandbookOfPracticalLogicLean/Chapter2/Extra.lean
@@ -1,0 +1,288 @@
+import Lean
+import Batteries.Tactic.Lint.Frontend
+import Mathlib.Util.CompileInductive
+import Mathlib.Tactic
+
+
+set_option autoImplicit false
+
+
+/--
+  The type of formulas.
+-/
+inductive Formula_ : Type
+  | false_ : Formula_
+  | true_ : Formula_
+  | atom_ : String → Formula_
+  | not_ : Formula_ → Formula_
+  | and_ : Formula_ → Formula_ → Formula_
+  | or_ : Formula_ → Formula_ → Formula_
+  | imp_ : Formula_ → Formula_ → Formula_
+  | iff_ : Formula_ → Formula_ → Formula_
+  | forall_ : String → Formula_ → Formula_
+  | exists_ : String → Formula_ → Formula_
+  deriving Inhabited, DecidableEq, Repr
+
+compile_inductive% Formula_
+
+
+/--
+  The string representation of formulas.
+-/
+def Formula_.toString :
+  Formula_ → String
+  | false_ => "F."
+  | true_ => "T."
+  | atom_ X => s! "{X}"
+  | not_ phi => s! "¬ {phi.toString}"
+  | and_ phi psi => s! "({phi.toString} ∧ {psi.toString})"
+  | or_ phi psi => s! "({phi.toString} ∨ {psi.toString})"
+  | imp_ phi psi => s! "({phi.toString} → {psi.toString})"
+  | iff_ phi psi => s! "({phi.toString} ↔ {psi.toString})"
+  | forall_ x phi => s! "(∀. {x} {phi.toString})"
+  | exists_ x phi => s! "(∃. {x} {phi.toString})"
+
+instance : ToString Formula_ :=
+  { toString := Formula_.toString }
+
+#eval (Formula_.atom_ "P").toString
+
+
+open Lean Elab Meta
+
+declare_syntax_cat formula
+
+
+syntax "F." : formula
+syntax "T." : formula
+syntax ident : formula
+syntax "~" formula : formula
+syntax "(" formula "/\\" formula ")" : formula
+syntax "(" formula "\\/" formula ")" : formula
+syntax "(" formula "->" formula ")" : formula
+syntax "(" formula "<->" formula ")" : formula
+syntax "(" "A." ident formula ")" : formula
+syntax "(" "E." ident formula ")" : formula
+
+
+partial def elabFormula : Syntax → MetaM Expr
+  | `(formula| F.) => mkAppM ``Formula_.false_ #[]
+
+  | `(formula| T.) => mkAppM ``Formula_.true_ #[]
+
+  | `(formula| $X:ident) => do
+    let X' : Expr := Lean.mkStrLit X.getId.toString
+    mkAppM ``Formula_.atom_ #[X']
+
+  | `(formula| ~ $phi) => do
+    let phi' : Expr ← elabFormula phi
+    mkAppM ``Formula_.not_ #[phi']
+
+  | `(formula| ($phi:formula /\ $psi:formula)) => do
+    let phi' : Expr ← elabFormula phi
+    let psi' : Expr ← elabFormula psi
+    mkAppM ``Formula_.and_ #[phi', psi']
+
+  | `(formula| ($phi:formula \/ $psi:formula)) => do
+    let phi' : Expr ← elabFormula phi
+    let psi' : Expr ← elabFormula psi
+    mkAppM ``Formula_.or_ #[phi', psi']
+
+  | `(formula| ($phi:formula -> $psi:formula)) => do
+    let phi' : Expr ← elabFormula phi
+    let psi' : Expr ← elabFormula psi
+    mkAppM ``Formula_.imp_ #[phi', psi']
+
+  | `(formula| ($phi:formula <-> $psi:formula)) => do
+    let phi' : Expr ← elabFormula phi
+    let psi' : Expr ← elabFormula psi
+    mkAppM ``Formula_.iff_ #[phi', psi']
+
+  | `(formula| (A. $x:ident $phi)) => do
+    let x' : Expr := Lean.mkStrLit x.getId.toString
+    let phi' : Expr ← elabFormula phi
+    mkAppM ``Formula_.forall_ #[x', phi']
+
+  | `(formula| (E. $x:ident $phi)) => do
+    let x' : Expr := Lean.mkStrLit x.getId.toString
+    let phi' : Expr ← elabFormula phi
+    mkAppM ``Formula_.exists_ #[x', phi']
+
+  | _ => throwUnsupportedSyntax
+
+
+elab "(Formula_|" p:formula ")" : term => elabFormula p
+
+
+#check (Formula_| F. )
+#check (Formula_| T. )
+#check (Formula_| P )
+#check (Formula_| ~ P )
+#check (Formula_| (P /\ Q) )
+#check (Formula_| (P \/ Q) )
+#check (Formula_| (P -> Q) )
+#check (Formula_| (P <-> Q) )
+#check (Formula_| ( A. x P ) )
+#check (Formula_| ( E. x P ) )
+
+
+
+open Formula_
+
+def Formula_.map_atoms
+  (f : String → Formula_) :
+  Formula_ → Formula_
+  | false_ => false_
+  | true_ => true_
+  | atom_ X => f X
+  | not_ phi => not_ (phi.map_atoms f)
+  | and_ phi psi => and_ (phi.map_atoms f) (psi.map_atoms f)
+  | or_ phi psi => or_ (phi.map_atoms f) (psi.map_atoms f)
+  | imp_ phi psi => imp_ (phi.map_atoms f) (psi.map_atoms f)
+  | iff_ phi psi => iff_ (phi.map_atoms f) (psi.map_atoms f)
+  | forall_ x phi => forall_ x (phi.map_atoms f)
+  | exists_ x phi => forall_ x (phi.map_atoms f)
+
+
+-- Applies function f to all of the atoms of the formula, from right to left.
+def Formula_.foldr_atoms
+  {α : Type}
+  (f : String → α → α)
+  (init : α) :
+  Formula_ → α
+  | false_
+  | true_ => init
+  | atom_ X => f X init
+  | not_ phi => phi.foldr_atoms f init
+  | and_ phi psi
+  | or_ phi psi
+  | imp_ phi psi
+  | iff_ phi psi => phi.foldr_atoms f (psi.foldr_atoms f init)
+  | forall_ _ phi
+  | exists_ _ phi => phi.foldr_atoms f init
+
+
+def atom_occurs_in
+  (A : String) :
+  Formula_ → Prop
+  | false_
+  | true_ => False
+  | atom_ X => A = X
+  | not_ phi => atom_occurs_in A phi
+  | and_ phi psi
+  | or_ phi psi
+  | imp_ phi psi
+  | iff_ phi psi => atom_occurs_in A phi ∨ atom_occurs_in A psi
+  | forall_ _ phi
+  | exists_ _ phi => atom_occurs_in A phi
+
+
+def PropValuation : Type := String → Prop
+  deriving Inhabited
+
+
+def eval
+  (V : PropValuation) :
+  Formula_ → Prop
+  | false_ => False
+  | true_ => True
+  | atom_ X => V X
+  | not_ phi => ¬ eval V phi
+  | and_ phi psi => eval V phi ∧ eval V psi
+  | or_ phi psi => eval V phi ∨ eval V psi
+  | imp_ phi psi => eval V phi → eval V psi
+  | iff_ phi psi => eval V phi ↔ eval V psi
+  | forall_ _ phi
+  | exists_ _ phi => eval V phi
+
+instance
+  (V : PropValuation)
+  [DecidablePred V]
+  (F : Formula_) :
+  Decidable (eval V F) :=
+  by
+  induction F
+  all_goals
+    simp only [eval]
+    infer_instance
+
+
+def eval_opt
+  (V : PropValuation) :
+  Formula_ → Option Prop
+  | false_ => some False
+  | true_ => some True
+  | atom_ X => some (V X)
+  | not_ phi => do
+    let val_phi ← eval_opt V phi
+    ¬ val_phi
+  | and_ phi psi => do
+    let val_phi ← eval_opt V phi
+    let val_psi ← eval_opt V psi
+    val_phi ∧ val_psi
+  | or_ phi psi => do
+    let val_phi ← eval_opt V phi
+    let val_psi ← eval_opt V psi
+    val_phi ∨ val_psi
+  | imp_ phi psi => do
+    let val_phi ← eval_opt V phi
+    let val_psi ← eval_opt V psi
+    val_phi → val_psi
+  | iff_ phi psi => do
+    let val_phi ← eval_opt V phi
+    let val_psi ← eval_opt V psi
+    val_phi ↔ val_psi
+  | forall_ _ _
+  | exists_ _ _ => none
+
+
+def Formula_.is_prop :
+  Formula_ → Prop
+  | false_
+  | true_
+  | atom_ _ => True
+  | not_ phi => phi.is_prop
+  | and_ phi psi
+  | or_ phi psi
+  | imp_ phi psi
+  | iff_ phi psi => phi.is_prop ∧ psi.is_prop
+  | forall_ _ _
+  | exists_ _ _ => False
+
+
+lemma is_prop_imp_eval_opt_eq_some_eval
+  (F : Formula_)
+  (V : PropValuation)
+  (h1 : F.is_prop) :
+  eval_opt V F = some (eval V F) :=
+  by
+  induction F
+  case false_ | true_ | atom_ X =>
+    unfold eval_opt
+    unfold eval
+    rfl
+  case not_ phi ih =>
+    unfold is_prop at h1
+
+    simp only [eval_opt]
+    rewrite [ih h1]
+    simp only [eval]
+    simp
+  case
+      and_ phi psi phi_ih psi_ih
+    | or_ phi psi phi_ih psi_ih
+    | imp_ phi psi phi_ih psi_ih
+    | iff_ phi psi phi_ih psi_ih =>
+    unfold is_prop at h1
+    obtain ⟨h1_left, h1_right⟩ := h1
+
+    simp only [eval_opt]
+    rewrite [phi_ih h1_left]
+    rewrite [psi_ih h1_right]
+    simp only [eval]
+    simp
+  case
+      forall_ x phi ih
+    | exists_ x phi ih =>
+      unfold is_prop at h1
+      contradiction
