HandbookOfPracticalLogicLean/Chapter2/Formula.lean
@@ -1,0 +1,115 @@
+import Lean
+import Batteries.Tactic.Lint.Frontend
+import Mathlib.Util.CompileInductive
+import Mathlib.Tactic
+
+
+set_option autoImplicit false
+
+
+/--
+  The type of formulas.
+-/
+inductive Formula_ : Type
+  | false_ : Formula_
+  | true_ : Formula_
+  | atom_ : String → Formula_
+  | not_ : Formula_ → Formula_
+  | and_ : Formula_ → Formula_ → Formula_
+  | or_ : Formula_ → Formula_ → Formula_
+  | imp_ : Formula_ → Formula_ → Formula_
+  | iff_ : Formula_ → Formula_ → Formula_
+  deriving Inhabited, DecidableEq, Repr
+
+compile_inductive% Formula_
+
+
+/--
+  The string representation of formulas.
+-/
+def Formula_.toString :
+  Formula_ → String
+  | false_ => "F."
+  | true_ => "T."
+  | atom_ X => s! "{X}"
+  | not_ phi => s! "¬ {phi.toString}"
+  | and_ phi psi => s! "({phi.toString} ∧ {psi.toString})"
+  | or_ phi psi => s! "({phi.toString} ∨ {psi.toString})"
+  | imp_ phi psi => s! "({phi.toString} → {psi.toString})"
+  | iff_ phi psi => s! "({phi.toString} ↔ {psi.toString})"
+
+instance : ToString Formula_ :=
+  { toString := Formula_.toString }
+
+
+open Lean Elab Meta
+
+declare_syntax_cat formula
+
+
+syntax "F." : formula
+syntax "T." : formula
+syntax ident : formula
+syntax "~" formula : formula
+syntax "(" formula "/\\" formula ")" : formula
+syntax "(" formula "\\/" formula ")" : formula
+syntax "(" formula "->" formula ")" : formula
+syntax "(" formula "<->" formula ")" : formula
+
+
+partial def elabFormula : Syntax → MetaM Expr
+  | `(formula| F.) => mkAppM ``Formula_.false_ #[]
+
+  | `(formula| T.) => mkAppM ``Formula_.true_ #[]
+
+  | `(formula| $X:ident) => do
+    let X' : Expr := Lean.mkStrLit X.getId.toString
+    mkAppM ``Formula_.atom_ #[X']
+
+  | `(formula| ~ $phi) => do
+    let phi' : Expr ← elabFormula phi
+    mkAppM ``Formula_.not_ #[phi']
+
+  | `(formula| ($phi:formula /\ $psi:formula)) => do
+    let phi' : Expr ← elabFormula phi
+    let psi' : Expr ← elabFormula psi
+    mkAppM ``Formula_.and_ #[phi', psi']
+
+  | `(formula| ($phi:formula \/ $psi:formula)) => do
+    let phi' : Expr ← elabFormula phi
+    let psi' : Expr ← elabFormula psi
+    mkAppM ``Formula_.or_ #[phi', psi']
+
+  | `(formula| ($phi:formula -> $psi:formula)) => do
+    let phi' : Expr ← elabFormula phi
+    let psi' : Expr ← elabFormula psi
+    mkAppM ``Formula_.imp_ #[phi', psi']
+
+  | `(formula| ($phi:formula <-> $psi:formula)) => do
+    let phi' : Expr ← elabFormula phi
+    let psi' : Expr ← elabFormula psi
+    mkAppM ``Formula_.iff_ #[phi', psi']
+
+  | _ => throwUnsupportedSyntax
+
+
+elab "(Formula_|" p:formula ")" : term => elabFormula p
+
+
+#check (Formula_| F. )
+#check (Formula_| T. )
+#check (Formula_| P )
+#check (Formula_| ~ P )
+#check (Formula_| (P /\ Q) )
+#check (Formula_| (P \/ Q) )
+#check (Formula_| (P -> Q) )
+#check (Formula_| (P <-> Q) )
+
+#eval (Formula_| F. ).toString
+#eval (Formula_| T. ).toString
+#eval (Formula_| P ).toString
+#eval (Formula_| ~ P ).toString
+#eval (Formula_| (P /\ Q) ).toString
+#eval (Formula_| (P \/ Q) ).toString
+#eval (Formula_| (P -> Q) ).toString
+#eval (Formula_| (P <-> Q) ).toString
